memory_ops_solvers_impl_soundness_misc.v
@@ -1,0 +1,389 @@
+Require Import Arith.  
+Require Import Nat. 
+Require Import Bool.
+Require Import bbv.Word. 
+Require Import Coq.NArith.NArith.
+Require Import List.
+Import ListNotations.
+Require Import Coq.Logic.FunctionalExtensionality.
+
+Require Import FORVES.constants.
+Import Constants.
+
+Require Import FORVES.program.
+Import Program.
+
+Require Import FORVES.execution_state.
+Import ExecutionState.
+
+Require Import FORVES.stack_operation_instructions.
+Import StackOpInstrs.
+
+Require Import FORVES.misc.
+Import Misc.
+
+Require Import FORVES.symbolic_state.
+Import SymbolicState.
+
+Require Import FORVES.symbolic_state_eval.
+Import SymbolicStateEval.
+
+Require Import FORVES.symbolic_state_eval_facts.
+Import SymbolicStateEvalFacts.
+
+Require Import FORVES.valid_symbolic_state.
+Import ValidSymbolicState.
+
+Require Import FORVES.memory_ops_solvers.
+Import MemoryOpsSolvers.
+
+Require Import FORVES.memory_ops_solvers_impl.
+Import MemoryOpsSolversImpl.
+
+Require Import FORVES.symbolic_state_cmp.
+Import SymbolicStateCmp.
+
+Require Import FORVES.symbolic_execution_soundness.
+Import SymbolicExecutionSoundness.
+
+Require Import storage_ops_solvers_impl_soundness.
+Import StorageOpsSolversImplSoundness.
+
+Module MemoryOpsSolversImplSoundnessMisc.
+
+  Ltac assoc_ones :=
+  intros;
+  repeat rewrite N.add_assoc;
+  reflexivity.
+
+Lemma assoc_ones_2 : forall x, (x+1+1 = x+(1+1))%N. Proof. assoc_ones. Qed.
+Lemma assoc_ones_3 : forall x, (x+1+1+1 = x+(1+1+1))%N. Proof. assoc_ones. Qed.
+Lemma assoc_ones_4 : forall x, (x+1+1+1+1 = x+(1+1+1+1))%N. Proof. assoc_ones. Qed.
+Lemma assoc_ones_5 : forall x, (x+1+1+1+1+1 = x+(1+1+1+1+1))%N. Proof. assoc_ones. Qed.
+Lemma assoc_ones_6 : forall x, (x+1+1+1+1+1+1 = x+(1+1+1+1+1+1))%N. Proof. assoc_ones. Qed.
+Lemma assoc_ones_7 : forall x, (x+1+1+1+1+1+1+1 = x+(1+1+1+1+1+1+1))%N. Proof. assoc_ones. Qed.
+Lemma assoc_ones_8 : forall x, (x+1+1+1+1+1+1+1+1 = x+(1+1+1+1+1+1+1+1))%N. Proof. assoc_ones. Qed.
+Lemma assoc_ones_9 : forall x, (x+1+1+1+1+1+1+1+1+1 = x+(1+1+1+1+1+1+1+1+1))%N. Proof. assoc_ones. Qed.
+Lemma assoc_ones_10: forall x, (x+1+1+1+1+1+1+1+1+1+1 = x+(1+1+1+1+1+1+1+1+1+1))%N. Proof. assoc_ones. Qed.
+Lemma assoc_ones_11: forall x, (x+1+1+1+1+1+1+1+1+1+1+1 = x+(1+1+1+1+1+1+1+1+1+1+1))%N. Proof. assoc_ones. Qed.
+Lemma assoc_ones_12: forall x, (x+1+1+1+1+1+1+1+1+1+1+1+1 = x+(1+1+1+1+1+1+1+1+1+1+1+1))%N. Proof. assoc_ones. Qed.
+Lemma assoc_ones_13: forall x, (x+1+1+1+1+1+1+1+1+1+1+1+1+1 = x+(1+1+1+1+1+1+1+1+1+1+1+1+1))%N. Proof. assoc_ones. Qed.
+Lemma assoc_ones_14: forall x, (x+1+1+1+1+1+1+1+1+1+1+1+1+1+1 = x+(1+1+1+1+1+1+1+1+1+1+1+1+1+1))%N. Proof. assoc_ones. Qed.
+Lemma assoc_ones_15: forall x, (x+1+1+1+1+1+1+1+1+1+1+1+1+1+1+1 = x+(1+1+1+1+1+1+1+1+1+1+1+1+1+1+1))%N. Proof. assoc_ones. Qed.
+Lemma assoc_ones_16: forall x, (x+1+1+1+1+1+1+1+1+1+1+1+1+1+1+1+1 = x+(1+1+1+1+1+1+1+1+1+1+1+1+1+1+1+1))%N. Proof. assoc_ones. Qed.
+Lemma assoc_ones_17: forall x, (x+1+1+1+1+1+1+1+1+1+1+1+1+1+1+1+1+1 = x+(1+1+1+1+1+1+1+1+1+1+1+1+1+1+1+1+1))%N. Proof. assoc_ones. Qed.
+Lemma assoc_ones_18: forall x, (x+1+1+1+1+1+1+1+1+1+1+1+1+1+1+1+1+1+1 = x+(1+1+1+1+1+1+1+1+1+1+1+1+1+1+1+1+1+1))%N. Proof. assoc_ones. Qed.
+Lemma assoc_ones_19: forall x, (x+1+1+1+1+1+1+1+1+1+1+1+1+1+1+1+1+1+1+1 = x+(1+1+1+1+1+1+1+1+1+1+1+1+1+1+1+1+1+1+1))%N. Proof. assoc_ones. Qed.
+Lemma assoc_ones_20: forall x, (x+1+1+1+1+1+1+1+1+1+1+1+1+1+1+1+1+1+1+1+1 = x+(1+1+1+1+1+1+1+1+1+1+1+1+1+1+1+1+1+1+1+1))%N. Proof. assoc_ones. Qed.
+Lemma assoc_ones_21: forall x, (x+1+1+1+1+1+1+1+1+1+1+1+1+1+1+1+1+1+1+1+1+1 = x+(1+1+1+1+1+1+1+1+1+1+1+1+1+1+1+1+1+1+1+1+1))%N. Proof. assoc_ones. Qed.
+Lemma assoc_ones_22: forall x, (x+1+1+1+1+1+1+1+1+1+1+1+1+1+1+1+1+1+1+1+1+1+1 = x+(1+1+1+1+1+1+1+1+1+1+1+1+1+1+1+1+1+1+1+1+1+1))%N. Proof. assoc_ones. Qed.
+Lemma assoc_ones_23: forall x, (x+1+1+1+1+1+1+1+1+1+1+1+1+1+1+1+1+1+1+1+1+1+1+1 = x+(1+1+1+1+1+1+1+1+1+1+1+1+1+1+1+1+1+1+1+1+1+1+1))%N. Proof. assoc_ones. Qed.
+Lemma assoc_ones_24: forall x, (x+1+1+1+1+1+1+1+1+1+1+1+1+1+1+1+1+1+1+1+1+1+1+1+1 = x+(1+1+1+1+1+1+1+1+1+1+1+1+1+1+1+1+1+1+1+1+1+1+1+1))%N. Proof. assoc_ones. Qed.
+Lemma assoc_ones_25: forall x, (x+1+1+1+1+1+1+1+1+1+1+1+1+1+1+1+1+1+1+1+1+1+1+1+1+1 = x+(1+1+1+1+1+1+1+1+1+1+1+1+1+1+1+1+1+1+1+1+1+1+1+1+1))%N. Proof. assoc_ones. Qed.
+Lemma assoc_ones_26: forall x, (x+1+1+1+1+1+1+1+1+1+1+1+1+1+1+1+1+1+1+1+1+1+1+1+1+1+1 = x+(1+1+1+1+1+1+1+1+1+1+1+1+1+1+1+1+1+1+1+1+1+1+1+1+1+1))%N. Proof. assoc_ones. Qed.
+Lemma assoc_ones_27: forall x, (x+1+1+1+1+1+1+1+1+1+1+1+1+1+1+1+1+1+1+1+1+1+1+1+1+1+1+1 = x+(1+1+1+1+1+1+1+1+1+1+1+1+1+1+1+1+1+1+1+1+1+1+1+1+1+1+1))%N. Proof. assoc_ones. Qed.
+Lemma assoc_ones_28: forall x, (x+1+1+1+1+1+1+1+1+1+1+1+1+1+1+1+1+1+1+1+1+1+1+1+1+1+1+1+1 = x+(1+1+1+1+1+1+1+1+1+1+1+1+1+1+1+1+1+1+1+1+1+1+1+1+1+1+1+1))%N. Proof. assoc_ones. Qed.
+Lemma assoc_ones_29: forall x, (x+1+1+1+1+1+1+1+1+1+1+1+1+1+1+1+1+1+1+1+1+1+1+1+1+1+1+1+1+1 = x+(1+1+1+1+1+1+1+1+1+1+1+1+1+1+1+1+1+1+1+1+1+1+1+1+1+1+1+1+1))%N. Proof. assoc_ones. Qed.
+Lemma assoc_ones_30: forall x, (x+1+1+1+1+1+1+1+1+1+1+1+1+1+1+1+1+1+1+1+1+1+1+1+1+1+1+1+1+1+1 = x+(1+1+1+1+1+1+1+1+1+1+1+1+1+1+1+1+1+1+1+1+1+1+1+1+1+1+1+1+1+1))%N. Proof. assoc_ones. Qed.
+Lemma assoc_ones_31: forall x, (x+1+1+1+1+1+1+1+1+1+1+1+1+1+1+1+1+1+1+1+1+1+1+1+1+1+1+1+1+1+1+1 = x+(1+1+1+1+1+1+1+1+1+1+1+1+1+1+1+1+1+1+1+1+1+1+1+1+1+1+1+1+1+1+1))%N. Proof. assoc_ones. Qed.
+
+Lemma assoc_ones_32: forall x, (x+1+1+1+1+1+1+1+1+1+1+1+1+1+1+1+1+1+1+1+1+1+1+1+1+1+1+1+1+1+1+1+1 = x+(1+1+1+1+1+1+1+1+1+1+1+1+1+1+1+1+1+1+1+1+1+1+1+1+1+1+1+1+1+1+1+1))%N. Proof. assoc_ones. Qed.
+
+
+Lemma Reduce_ones_2 : (1+1 = 2)%N. Proof. intuition. Qed.
+Lemma Reduce_ones_3 : (1+1+1 = 3)%N. Proof. intuition. Qed.
+Lemma Reduce_ones_4 : (1+1+1+1 = 4)%N. Proof. intuition. Qed.
+Lemma Reduce_ones_5 : (1+1+1+1+1 = 5)%N. Proof. intuition. Qed.
+Lemma Reduce_ones_6 : (1+1+1+1+1+1 = 6)%N. Proof. intuition. Qed.
+Lemma Reduce_ones_7 : (1+1+1+1+1+1+1 = 7)%N. Proof. intuition. Qed.
+Lemma Reduce_ones_8 : (1+1+1+1+1+1+1+1 = 8)%N. Proof. intuition. Qed.
+Lemma Reduce_ones_9 : (1+1+1+1+1+1+1+1+1 = 9)%N. Proof. intuition. Qed.
+Lemma Reduce_ones_10: (1+1+1+1+1+1+1+1+1+1 = 10)%N. Proof. intuition. Qed.
+Lemma Reduce_ones_11: (1+1+1+1+1+1+1+1+1+1+1 = 11)%N. Proof. intuition. Qed.
+Lemma Reduce_ones_12: (1+1+1+1+1+1+1+1+1+1+1+1 = 12)%N. Proof. intuition. Qed.
+Lemma Reduce_ones_13: (1+1+1+1+1+1+1+1+1+1+1+1+1 = 13)%N. Proof. intuition. Qed.
+Lemma Reduce_ones_14: (1+1+1+1+1+1+1+1+1+1+1+1+1+1 = 14)%N. Proof. intuition. Qed.
+Lemma Reduce_ones_15: (1+1+1+1+1+1+1+1+1+1+1+1+1+1+1 = 15)%N. Proof. intuition. Qed.
+Lemma Reduce_ones_16: (1+1+1+1+1+1+1+1+1+1+1+1+1+1+1+1 = 16)%N. Proof. intuition. Qed.
+Lemma Reduce_ones_17: (1+1+1+1+1+1+1+1+1+1+1+1+1+1+1+1+1 = 17)%N. Proof. intuition. Qed.
+Lemma Reduce_ones_18: (1+1+1+1+1+1+1+1+1+1+1+1+1+1+1+1+1+1 = 18)%N. Proof. intuition. Qed.
+Lemma Reduce_ones_19: (1+1+1+1+1+1+1+1+1+1+1+1+1+1+1+1+1+1+1 = 19)%N. Proof. intuition. Qed.
+Lemma Reduce_ones_20: (1+1+1+1+1+1+1+1+1+1+1+1+1+1+1+1+1+1+1+1 = 20)%N. Proof. intuition. Qed.
+Lemma Reduce_ones_21: (1+1+1+1+1+1+1+1+1+1+1+1+1+1+1+1+1+1+1+1+1 = 21)%N. Proof. intuition. Qed.
+Lemma Reduce_ones_22: (1+1+1+1+1+1+1+1+1+1+1+1+1+1+1+1+1+1+1+1+1+1 = 22)%N. Proof. intuition. Qed.
+Lemma Reduce_ones_23: (1+1+1+1+1+1+1+1+1+1+1+1+1+1+1+1+1+1+1+1+1+1+1 = 23)%N. Proof. intuition. Qed.
+Lemma Reduce_ones_24: (1+1+1+1+1+1+1+1+1+1+1+1+1+1+1+1+1+1+1+1+1+1+1+1 = 24)%N. Proof. intuition. Qed.
+Lemma Reduce_ones_25: (1+1+1+1+1+1+1+1+1+1+1+1+1+1+1+1+1+1+1+1+1+1+1+1+1 = 25)%N. Proof. intuition. Qed.
+Lemma Reduce_ones_26: (1+1+1+1+1+1+1+1+1+1+1+1+1+1+1+1+1+1+1+1+1+1+1+1+1+1 = 26)%N. Proof. intuition. Qed.
+Lemma Reduce_ones_27: (1+1+1+1+1+1+1+1+1+1+1+1+1+1+1+1+1+1+1+1+1+1+1+1+1+1+1 = 27)%N. Proof. intuition. Qed.
+Lemma Reduce_ones_28: (1+1+1+1+1+1+1+1+1+1+1+1+1+1+1+1+1+1+1+1+1+1+1+1+1+1+1+1 = 28)%N. Proof. intuition. Qed.
+Lemma Reduce_ones_29: (1+1+1+1+1+1+1+1+1+1+1+1+1+1+1+1+1+1+1+1+1+1+1+1+1+1+1+1+1 = 29)%N. Proof. intuition. Qed.
+Lemma Reduce_ones_30: (1+1+1+1+1+1+1+1+1+1+1+1+1+1+1+1+1+1+1+1+1+1+1+1+1+1+1+1+1+1 = 30)%N. Proof. intuition. Qed.
+Lemma Reduce_ones_31: (1+1+1+1+1+1+1+1+1+1+1+1+1+1+1+1+1+1+1+1+1+1+1+1+1+1+1+1+1+1+1 = 31)%N. Proof. intuition. Qed.
+Lemma Reduce_ones_32: (1+1+1+1+1+1+1+1+1+1+1+1+1+1+1+1+1+1+1+1+1+1+1+1+1+1+1+1+1+1+1+1 = 32)%N. Proof. intuition. Qed.
+
+
+Lemma H_1_lt_32: (1<32)%N. Proof.  apply Nlt_in. intuition. Qed.
+Lemma H_2_lt_32: (2<32)%N. Proof.  apply Nlt_in. intuition. Qed.
+Lemma H_3_lt_32: (3<32)%N. Proof.  apply Nlt_in. intuition. Qed.
+Lemma H_4_lt_32: (4<32)%N. Proof.  apply Nlt_in. intuition. Qed.
+Lemma H_5_lt_32: (5<32)%N. Proof.  apply Nlt_in. intuition. Qed.
+Lemma H_6_lt_32: (6<32)%N. Proof.  apply Nlt_in. intuition. Qed.
+Lemma H_7_lt_32: (7<32)%N. Proof.  apply Nlt_in. intuition. Qed.
+Lemma H_8_lt_32: (8<32)%N. Proof.  apply Nlt_in. intuition. Qed.
+Lemma H_9_lt_32: (9<32)%N. Proof.  apply Nlt_in. intuition. Qed.
+Lemma H_10_lt_32: (10<32)%N. Proof.  apply Nlt_in. intuition. Qed.
+Lemma H_11_lt_32: (11<32)%N. Proof.  apply Nlt_in. intuition. Qed.
+Lemma H_12_lt_32: (12<32)%N. Proof.  apply Nlt_in. intuition. Qed.
+Lemma H_13_lt_32: (13<32)%N. Proof.  apply Nlt_in. intuition. Qed.
+Lemma H_14_lt_32: (14<32)%N. Proof.  apply Nlt_in. intuition. Qed.
+Lemma H_15_lt_32: (15<32)%N. Proof.  apply Nlt_in. intuition. Qed.
+Lemma H_16_lt_32: (16<32)%N. Proof.  apply Nlt_in. intuition. Qed.
+Lemma H_17_lt_32: (17<32)%N. Proof.  apply Nlt_in. intuition. Qed.
+Lemma H_18_lt_32: (18<32)%N. Proof.  apply Nlt_in. intuition. Qed.
+Lemma H_19_lt_32: (19<32)%N. Proof.  apply Nlt_in. intuition. Qed.
+Lemma H_20_lt_32: (20<32)%N. Proof.  apply Nlt_in. intuition. Qed.
+Lemma H_21_lt_32: (21<32)%N. Proof.  apply Nlt_in. intuition. Qed.
+Lemma H_22_lt_32: (22<32)%N. Proof.  apply Nlt_in. intuition. Qed.
+Lemma H_23_lt_32: (23<32)%N. Proof.  apply Nlt_in. intuition. Qed.
+Lemma H_24_lt_32: (24<32)%N. Proof.  apply Nlt_in. intuition. Qed.
+Lemma H_25_lt_32: (25<32)%N. Proof.  apply Nlt_in. intuition. Qed.
+Lemma H_26_lt_32: (26<32)%N. Proof.  apply Nlt_in. intuition. Qed.
+Lemma H_27_lt_32: (27<32)%N. Proof.  apply Nlt_in. intuition. Qed.
+Lemma H_28_lt_32: (28<32)%N. Proof.  apply Nlt_in. intuition. Qed.
+Lemma H_29_lt_32: (29<32)%N. Proof.  apply Nlt_in. intuition. Qed.
+Lemma H_30_lt_32: (30<32)%N. Proof.  apply Nlt_in. intuition. Qed.
+Lemma H_31_lt_32: (31<32)%N. Proof.  apply Nlt_in. intuition. Qed.
+
+Lemma H_1_le_31: (1<=31)%N. Proof.  apply N.lt_le_incl. apply Nlt_in. intuition. Qed.
+Lemma H_2_le_31: (2<=31)%N. Proof.  apply N.lt_le_incl. apply Nlt_in. intuition. Qed.
+Lemma H_3_le_31: (3<=31)%N. Proof.  apply N.lt_le_incl. apply Nlt_in. intuition. Qed.
+Lemma H_4_le_31: (4<=31)%N. Proof.  apply N.lt_le_incl. apply Nlt_in. intuition. Qed.
+Lemma H_5_le_31: (5<=31)%N. Proof.  apply N.lt_le_incl. apply Nlt_in. intuition. Qed.
+Lemma H_6_le_31: (6<=31)%N. Proof.  apply N.lt_le_incl. apply Nlt_in. intuition. Qed.
+Lemma H_7_le_31: (7<=31)%N. Proof.  apply N.lt_le_incl. apply Nlt_in. intuition. Qed.
+Lemma H_8_le_31: (8<=31)%N. Proof.  apply N.lt_le_incl. apply Nlt_in. intuition. Qed.
+Lemma H_9_le_31: (9<=31)%N. Proof.  apply N.lt_le_incl. apply Nlt_in. intuition. Qed.
+Lemma H_10_le_31: (10<=31)%N. Proof.  apply N.lt_le_incl. apply Nlt_in. intuition. Qed.
+Lemma H_11_le_31: (11<=31)%N. Proof.  apply N.lt_le_incl. apply Nlt_in. intuition. Qed.
+Lemma H_12_le_31: (12<=31)%N. Proof.  apply N.lt_le_incl. apply Nlt_in. intuition. Qed.
+Lemma H_13_le_31: (13<=31)%N. Proof.  apply N.lt_le_incl. apply Nlt_in. intuition. Qed.
+Lemma H_14_le_31: (14<=31)%N. Proof.  apply N.lt_le_incl. apply Nlt_in. intuition. Qed.
+Lemma H_15_le_31: (15<=31)%N. Proof.  apply N.lt_le_incl. apply Nlt_in. intuition. Qed.
+Lemma H_16_le_31: (16<=31)%N. Proof.  apply N.lt_le_incl. apply Nlt_in. intuition. Qed.
+Lemma H_17_le_31: (17<=31)%N. Proof.  apply N.lt_le_incl. apply Nlt_in. intuition. Qed.
+Lemma H_18_le_31: (18<=31)%N. Proof.  apply N.lt_le_incl. apply Nlt_in. intuition. Qed.
+Lemma H_19_le_31: (19<=31)%N. Proof.  apply N.lt_le_incl. apply Nlt_in. intuition. Qed.
+Lemma H_20_le_31: (20<=31)%N. Proof.  apply N.lt_le_incl. apply Nlt_in. intuition. Qed.
+Lemma H_21_le_31: (21<=31)%N. Proof.  apply N.lt_le_incl. apply Nlt_in. intuition. Qed.
+Lemma H_22_le_31: (22<=31)%N. Proof.  apply N.lt_le_incl. apply Nlt_in. intuition. Qed.
+Lemma H_23_le_31: (23<=31)%N. Proof.  apply N.lt_le_incl. apply Nlt_in. intuition. Qed.
+Lemma H_24_le_31: (24<=31)%N. Proof.  apply N.lt_le_incl. apply Nlt_in. intuition. Qed.
+Lemma H_25_le_31: (25<=31)%N. Proof.  apply N.lt_le_incl. apply Nlt_in. intuition. Qed.
+Lemma H_26_le_31: (26<=31)%N. Proof.  apply N.lt_le_incl. apply Nlt_in. intuition. Qed.
+Lemma H_27_le_31: (27<=31)%N. Proof.  apply N.lt_le_incl. apply Nlt_in. intuition. Qed.
+Lemma H_28_le_31: (28<=31)%N. Proof.  apply N.lt_le_incl. apply Nlt_in. intuition. Qed.
+Lemma H_29_le_31: (29<=31)%N. Proof.  apply N.lt_le_incl. apply Nlt_in. intuition. Qed.
+Lemma H_30_le_31: (30<=31)%N. Proof.  apply N.lt_le_incl. apply Nlt_in. intuition. Qed.
+Lemma H_31_le_31: (31<=31)%N. Proof.  intuition. Qed.
+
+
+Lemma do_not_overlap_mload_aux_0 n i k (offset offset' : word n) (H_i_lt_32: (i<32)%N) (H_o: (wordToN offset + 31 <? wordToN offset')%N || (wordToN offset' + k <? wordToN offset)%N = true):
+    (wordToN offset + i =? wordToN offset'= false)%N.
+Proof.
+  intros.
+  apply orb_prop in H_o.
+  destruct H_o.
+  + rewrite N.eqb_neq.
+    apply Nneq_in.
+    rewrite N.ltb_lt in H.
+    apply Nlt_out in H.
+    intuition.
+  + rewrite N.eqb_neq.
+    apply Nneq_in.
+    rewrite N.ltb_lt in H.
+    apply Nlt_out in H.
+    intuition.
+Qed.  
+
+Lemma do_not_overlap_mload_aux_1 n j i k (offset offset' : word n) (H_j_lt_k: (j<=k)%N) (H_j_lt_32: (j<32)%N) (H_i_lt_32: (i<32)%N) (H_o: (wordToN offset + 31 <? wordToN offset')%N || (wordToN offset' + k <? wordToN offset)%N = true):
+    (wordToN offset + i =? wordToN offset' + j = false)%N.
+Proof.
+  intros.
+  apply orb_prop in H_o.
+  destruct H_o.
+  + rewrite N.eqb_neq.
+    apply Nneq_in.
+    rewrite N.ltb_lt in H.
+    apply Nlt_out in H.
+    intuition.
+  + rewrite N.eqb_neq.
+    apply Nneq_in.
+    rewrite N.ltb_lt in H.
+    apply Nlt_out in H.
+    intuition.
+    Qed.
+
+Lemma do_not_overlap_mload_aux mem value' updates i offset offset' (H_i_lt_32: (i<32)%N) (H_not_overlap: (wordToN offset + 31 <? wordToN offset')%N || (wordToN offset' + 31 <? wordToN offset)%N = true):
+    (eval_common.EvalCommon.update_memory mem (U_MSTORE EVMWord offset' value' :: updates)) ((wordToN offset)+i)%N =
+    (eval_common.EvalCommon.update_memory mem  updates) ((wordToN (offset : EVMWord)+i))%N.
+Proof.
+  unfold eval_common.EvalCommon.update_memory.
+  remember ((fix update_memory (mem0 : memory) (updates0 : memory_updates EVMWord) {struct updates0} : memory := match updates0 with
+                                                                                                                 | [] => mem0
+                                                                                                                 | u :: us => eval_common.EvalCommon.update_memory' (update_memory mem0 us) u
+                                                                                                                 end) mem updates) as XX.
+  unfold eval_common.EvalCommon.update_memory'.
+  unfold concrete_interpreter.ConcreteInterpreter.mstore.
+  unfold concrete_interpreter.ConcreteInterpreter.mstore'.
+  unfold BytesInEVMWord.
+
+  rewrite assoc_ones_31.
+  rewrite Reduce_ones_31.
+
+  rewrite assoc_ones_30.
+  rewrite Reduce_ones_30.
+
+  rewrite assoc_ones_29.
+  rewrite Reduce_ones_29.
+
+  rewrite assoc_ones_28.
+  rewrite Reduce_ones_28.
+
+  rewrite assoc_ones_27.
+  rewrite Reduce_ones_27.
+
+  rewrite assoc_ones_26.
+  rewrite Reduce_ones_26.
+
+  rewrite assoc_ones_25.
+  rewrite Reduce_ones_25.
+
+  rewrite assoc_ones_24.
+  rewrite Reduce_ones_24.
+
+  rewrite assoc_ones_23.
+  rewrite Reduce_ones_23.
+
+  rewrite assoc_ones_22.
+  rewrite Reduce_ones_22.
+
+  rewrite assoc_ones_21.
+  rewrite Reduce_ones_21.
+
+  rewrite assoc_ones_20.
+  rewrite Reduce_ones_20.
+
+  rewrite assoc_ones_19.
+  rewrite Reduce_ones_19.
+
+  rewrite assoc_ones_18.
+  rewrite Reduce_ones_18.
+
+  rewrite assoc_ones_17.
+  rewrite Reduce_ones_17.
+
+  rewrite assoc_ones_16.
+  rewrite Reduce_ones_16.
+
+  rewrite assoc_ones_15.
+  rewrite Reduce_ones_15.
+
+  rewrite assoc_ones_14.
+  rewrite Reduce_ones_14.
+
+  rewrite assoc_ones_13.
+  rewrite Reduce_ones_13.
+
+  rewrite assoc_ones_12.
+  rewrite Reduce_ones_12.
+
+  rewrite assoc_ones_11.
+  rewrite Reduce_ones_11.
+
+  rewrite assoc_ones_10.
+  rewrite Reduce_ones_10.
+
+    rewrite assoc_ones_9.
+  rewrite Reduce_ones_9.
+
+  rewrite assoc_ones_8.
+  rewrite Reduce_ones_8.
+
+  rewrite assoc_ones_7.
+  rewrite Reduce_ones_7.
+
+  rewrite assoc_ones_6.
+  rewrite Reduce_ones_6.
+
+  rewrite assoc_ones_5.
+  rewrite Reduce_ones_5.
+
+  rewrite assoc_ones_4.
+  rewrite Reduce_ones_4.
+
+  rewrite assoc_ones_3.
+  rewrite Reduce_ones_3.
+
+  rewrite assoc_ones_2.
+  rewrite Reduce_ones_2.
+
+
+
+  rewrite (do_not_overlap_mload_aux_0 EVMWordSize i 31%N offset offset' H_i_lt_32 H_not_overlap).
+  rewrite (do_not_overlap_mload_aux_1 EVMWordSize 1%N i 31%N  offset offset' H_1_le_31 H_1_lt_32 H_i_lt_32 H_not_overlap).
+  rewrite (do_not_overlap_mload_aux_1 EVMWordSize 2%N i 31%N offset offset' H_2_le_31 H_2_lt_32 H_i_lt_32 H_not_overlap).
+  rewrite (do_not_overlap_mload_aux_1 EVMWordSize 3%N i 31%N offset offset' H_3_le_31 H_3_lt_32 H_i_lt_32 H_not_overlap).
+  rewrite (do_not_overlap_mload_aux_1 EVMWordSize 4%N i  31%N offset offset' H_4_le_31 H_4_lt_32 H_i_lt_32 H_not_overlap).
+  rewrite (do_not_overlap_mload_aux_1 EVMWordSize 5%N i  31%N offset offset' H_5_le_31 H_5_lt_32 H_i_lt_32 H_not_overlap).
+  rewrite (do_not_overlap_mload_aux_1 EVMWordSize 6%N i  31%N offset offset' H_6_le_31 H_6_lt_32 H_i_lt_32 H_not_overlap).
+  rewrite (do_not_overlap_mload_aux_1 EVMWordSize 7%N i  31%N offset offset' H_7_le_31 H_7_lt_32 H_i_lt_32 H_not_overlap).
+  rewrite (do_not_overlap_mload_aux_1 EVMWordSize 8%N i  31%N offset offset' H_8_le_31 H_8_lt_32 H_i_lt_32 H_not_overlap).
+  rewrite (do_not_overlap_mload_aux_1 EVMWordSize 9%N i  31%N offset offset' H_9_le_31 H_9_lt_32 H_i_lt_32 H_not_overlap).
+  rewrite (do_not_overlap_mload_aux_1 EVMWordSize 10%N i  31%N offset offset' H_10_le_31 H_10_lt_32 H_i_lt_32 H_not_overlap).
+  rewrite (do_not_overlap_mload_aux_1 EVMWordSize 11%N i  31%N offset offset' H_11_le_31 H_11_lt_32 H_i_lt_32 H_not_overlap).
+  rewrite (do_not_overlap_mload_aux_1 EVMWordSize 12%N i  31%N offset offset' H_12_le_31 H_12_lt_32 H_i_lt_32 H_not_overlap).
+  rewrite (do_not_overlap_mload_aux_1 EVMWordSize 13%N i  31%N offset offset' H_13_le_31 H_13_lt_32 H_i_lt_32 H_not_overlap).
+  rewrite (do_not_overlap_mload_aux_1 EVMWordSize 14%N i  31%N offset offset' H_14_le_31 H_14_lt_32 H_i_lt_32 H_not_overlap).
+  rewrite (do_not_overlap_mload_aux_1 EVMWordSize 15%N i  31%N offset offset' H_15_le_31 H_15_lt_32 H_i_lt_32 H_not_overlap).
+  rewrite (do_not_overlap_mload_aux_1 EVMWordSize 16%N i  31%N offset offset' H_16_le_31 H_16_lt_32 H_i_lt_32 H_not_overlap).
+  rewrite (do_not_overlap_mload_aux_1 EVMWordSize 17%N i  31%N offset offset' H_17_le_31 H_17_lt_32 H_i_lt_32 H_not_overlap).
+  rewrite (do_not_overlap_mload_aux_1 EVMWordSize 18%N i  31%N offset offset' H_18_le_31 H_18_lt_32 H_i_lt_32 H_not_overlap).
+  rewrite (do_not_overlap_mload_aux_1 EVMWordSize 19%N i  31%N offset offset' H_19_le_31 H_19_lt_32 H_i_lt_32 H_not_overlap).
+  rewrite (do_not_overlap_mload_aux_1 EVMWordSize 20%N i  31%N offset offset' H_20_le_31 H_20_lt_32 H_i_lt_32 H_not_overlap).
+  rewrite (do_not_overlap_mload_aux_1 EVMWordSize 21%N i  31%N offset offset' H_21_le_31 H_21_lt_32 H_i_lt_32 H_not_overlap).
+  rewrite (do_not_overlap_mload_aux_1 EVMWordSize 22%N i  31%N offset offset' H_22_le_31 H_22_lt_32 H_i_lt_32 H_not_overlap).
+  rewrite (do_not_overlap_mload_aux_1 EVMWordSize 23%N i  31%N offset offset' H_23_le_31 H_23_lt_32 H_i_lt_32 H_not_overlap).
+  rewrite (do_not_overlap_mload_aux_1 EVMWordSize 24%N i  31%N offset offset' H_24_le_31 H_24_lt_32 H_i_lt_32 H_not_overlap).
+  rewrite (do_not_overlap_mload_aux_1 EVMWordSize 25%N i  31%N offset offset' H_25_le_31 H_25_lt_32 H_i_lt_32 H_not_overlap).
+  rewrite (do_not_overlap_mload_aux_1 EVMWordSize 26%N i  31%N offset offset' H_26_le_31 H_26_lt_32 H_i_lt_32 H_not_overlap).
+  rewrite (do_not_overlap_mload_aux_1 EVMWordSize 27%N i  31%N offset offset' H_27_le_31 H_27_lt_32 H_i_lt_32 H_not_overlap).
+  rewrite (do_not_overlap_mload_aux_1 EVMWordSize 28%N i  31%N offset offset' H_28_le_31 H_28_lt_32 H_i_lt_32 H_not_overlap).
+  rewrite (do_not_overlap_mload_aux_1 EVMWordSize 29%N i  31%N offset offset' H_29_le_31 H_29_lt_32 H_i_lt_32 H_not_overlap).
+  rewrite (do_not_overlap_mload_aux_1 EVMWordSize 30%N i  31%N offset offset' H_30_le_31 H_30_lt_32 H_i_lt_32 H_not_overlap).
+  rewrite (do_not_overlap_mload_aux_1 EVMWordSize 31%N i  31%N offset offset' H_31_le_31 H_31_lt_32 H_i_lt_32 H_not_overlap).
+  reflexivity.
+Qed.
+
+Lemma do_not_overlap_mload_aux' mem value' updates i offset offset' (H_i_lt_32: (i<32)%N) (H_not_overlap: (wordToN offset + 31 <? wordToN offset')%N || (wordToN offset' + 0 <? wordToN offset)%N = true):
+    (eval_common.EvalCommon.update_memory mem (U_MSTORE8 EVMWord offset' value' :: updates)) ((wordToN offset)+i)%N =
+    (eval_common.EvalCommon.update_memory mem  updates) ((wordToN (offset : EVMWord)+i))%N.
+Proof.
+  unfold eval_common.EvalCommon.update_memory.
+  remember ((fix update_memory (mem0 : memory) (updates0 : memory_updates EVMWord) {struct updates0} : memory := match updates0 with
+                                                                                                                 | [] => mem0
+                                                                                                                 | u :: us => eval_common.EvalCommon.update_memory' (update_memory mem0 us) u
+                                                                                                                 end) mem updates) as XX.
+  unfold eval_common.EvalCommon.update_memory'.
+  unfold concrete_interpreter.ConcreteInterpreter.mstore.
+  unfold concrete_interpreter.ConcreteInterpreter.mstore'.
+
+  
+
+
+
+  rewrite (do_not_overlap_mload_aux_0 EVMWordSize i 0%N offset offset' H_i_lt_32 H_not_overlap).
+  reflexivity.
+Qed.
+
+End MemoryOpsSolversImplSoundnessMisc.
